src/Common.v
@@ -483,9 +483,9 @@ Ltac higher_order_1_reflexivity :=
         | sym_higher_order_1_reflexivity' ].
 
 Ltac higher_order_1_f_reflexivity :=
-  let a := match goal with |- ?R (?g ?a) (?g (?f ?x)) => constr:(a) end in
-  let f := match goal with |- ?R (?g ?a) (?g (?f ?x)) => constr:(f) end in
-  let x := match goal with |- ?R (?g ?a) (?g (?f ?x)) => constr:(x) end in
+  let a := match goal with |- ?R (?g ?a) (?g' (?f ?x)) => constr:(a) end in
+  let f := match goal with |- ?R (?g ?a) (?g' (?f ?x)) => constr:(f) end in
+  let x := match goal with |- ?R (?g ?a) (?g' (?f ?x)) => constr:(x) end in
   let a' := (eval pattern x in a) in
   let f' := match a' with ?f' _ => constr:(f') end in
   unify f f';
@@ -521,10 +521,10 @@ Ltac higher_order_2_reflexivity :=
         | sym_higher_order_2_reflexivity' ].
 
 Ltac higher_order_2_f_reflexivity :=
-  let x := match goal with |- ?R (?g ?x) (?g (?f ?a ?b)) => constr:(x) end in
-  let f := match goal with |- ?R (?g ?x) (?g (?f ?a ?b)) => constr:(f) end in
-  let a := match goal with |- ?R (?g ?x) (?g (?f ?a ?b)) => constr:(a) end in
-  let b := match goal with |- ?R (?g ?x) (?g (?f ?a ?b)) => constr:(b) end in
+  let x := match goal with |- ?R (?g ?x) (?g' (?f ?a ?b)) => constr:(x) end in
+  let f := match goal with |- ?R (?g ?x) (?g' (?f ?a ?b)) => constr:(f) end in
+  let a := match goal with |- ?R (?g ?x) (?g' (?f ?a ?b)) => constr:(a) end in
+  let b := match goal with |- ?R (?g ?x) (?g' (?f ?a ?b)) => constr:(b) end in
   let x' := (eval pattern a, b in x) in
   let f' := match x' with ?f' _ _ => constr:(f') end in
   unify f f';
@@ -544,11 +544,11 @@ Ltac higher_order_3_reflexivity :=
     solve [apply reflexivity].
 
 Ltac higher_order_3_f_reflexivity :=
-  let x := match goal with |- ?R (?g ?x) (?g (?f ?a ?b ?c)) => constr:(x) end in
-  let f := match goal with |- ?R (?g ?x) (?g (?f ?a ?b ?c)) => constr:(f) end in
-  let a := match goal with |- ?R (?g ?x) (?g (?f ?a ?b ?c)) => constr:(a) end in
-  let b := match goal with |- ?R (?g ?x) (?g (?f ?a ?b ?c)) => constr:(b) end in
-  let c := match goal with |- ?R (?g ?x) (?g (?f ?a ?b ?c)) => constr:(c) end in
+  let x := match goal with |- ?R (?g ?x) (?g' (?f ?a ?b ?c)) => constr:(x) end in
+  let f := match goal with |- ?R (?g ?x) (?g' (?f ?a ?b ?c)) => constr:(f) end in
+  let a := match goal with |- ?R (?g ?x) (?g' (?f ?a ?b ?c)) => constr:(a) end in
+  let b := match goal with |- ?R (?g ?x) (?g' (?f ?a ?b ?c)) => constr:(b) end in
+  let c := match goal with |- ?R (?g ?x) (?g' (?f ?a ?b ?c)) => constr:(c) end in
   let x' := (eval pattern a, b, c in x) in
   let f' := match x' with ?f' _ _ _ => constr:(f') end in
   unify f f';
@@ -569,12 +569,12 @@ Ltac higher_order_4_reflexivity :=
     solve [apply reflexivity].
 
 Ltac higher_order_4_f_reflexivity :=
-  let x := match goal with |- ?R (?g ?x) (?g (?f ?a ?b ?c ?d)) => constr:(x) end in
-  let f := match goal with |- ?R (?g ?x) (?g (?f ?a ?b ?c ?d)) => constr:(f) end in
-  let a := match goal with |- ?R (?g ?x) (?g (?f ?a ?b ?c ?d)) => constr:(a) end in
-  let b := match goal with |- ?R (?g ?x) (?g (?f ?a ?b ?c ?d)) => constr:(b) end in
-  let c := match goal with |- ?R (?g ?x) (?g (?f ?a ?b ?c ?d)) => constr:(c) end in
-  let d := match goal with |- ?R (?g ?x) (?g (?f ?a ?b ?c ?d)) => constr:(d) end in
+  let x := match goal with |- ?R (?g ?x) (?g' (?f ?a ?b ?c ?d)) => constr:(x) end in
+  let f := match goal with |- ?R (?g ?x) (?g' (?f ?a ?b ?c ?d)) => constr:(f) end in
+  let a := match goal with |- ?R (?g ?x) (?g' (?f ?a ?b ?c ?d)) => constr:(a) end in
+  let b := match goal with |- ?R (?g ?x) (?g' (?f ?a ?b ?c ?d)) => constr:(b) end in
+  let c := match goal with |- ?R (?g ?x) (?g' (?f ?a ?b ?c ?d)) => constr:(c) end in
+  let d := match goal with |- ?R (?g ?x) (?g' (?f ?a ?b ?c ?d)) => constr:(d) end in
   let x' := (eval pattern a, b, c, d in x) in
   let f' := match x' with ?f' _ _ _ _ => constr:(f') end in
   unify f f';
@@ -583,10 +583,10 @@ Ltac higher_order_4_f_reflexivity :=
 
 Ltac higher_order_reflexivity :=
   match goal with
-    | |- ?R (?g ?x) (?g (?f ?a ?b ?c ?d)) =>  higher_order_4_f_reflexivity
-    | |- ?R (?g ?x) (?g (?f ?a ?b ?c))    =>  higher_order_3_f_reflexivity
-    | |- ?R (?g ?x) (?g (?f ?a ?b))       =>  higher_order_2_f_reflexivity
-    | |- ?R (?g ?x) (?g (?f ?a))          =>  higher_order_1_f_reflexivity
+    | |- ?R (?g ?x) (?g' (?f ?a ?b ?c ?d)) =>  higher_order_4_f_reflexivity
+    | |- ?R (?g ?x) (?g' (?f ?a ?b ?c))    =>  higher_order_3_f_reflexivity
+    | |- ?R (?g ?x) (?g' (?f ?a ?b))       =>  higher_order_2_f_reflexivity
+    | |- ?R (?g ?x) (?g' (?f ?a))          =>  higher_order_1_f_reflexivity
 
     | |- ?R ?x (?f ?a ?b ?c ?d)           =>  higher_order_4_reflexivity
     | |- ?R ?x (?f ?a ?b ?c)              =>  higher_order_3_reflexivity
